# 4.3 Exercises

### 4.3.1

Exercise 4.3.1 : The following is a grammar for regular expressions over symbols a and b only, using + in place of | for union, to avoid conflict with the use of vertical bar as a metasymbol in grammars:

    rexpr -> rexpr + rterm | rterm
    rterm -> rterm rfactor | rfactor
    rfactor -> rfactor \* | rprimary
    rprimary -> a | b

a) Left factor this grammar.

b) Does left factoring make the grammar suitable for top-down parsing?

c) In addition to left factoring, eliminate left recursion from the original grammar.

d) Is the resulting grammar suitable for top-down parsing?

#### Answer

1. left factoring not needed.
2. No
3. Eliminating left recursion:
        
           rexpr -> rterm A
               A -> + rterm A | ε
           rterm -> rfactor B
               B -> rfactor B | ε
         rfactor -> rprimary C
               C -> * C | ε
        rprimary -> a | b

4. Yes

### 4.3.2

Repeat Exercise 4.3.1 on the following grammars:

a) The grammar of Exercise 4.2.1.

b) The grammar of Exercise 4.2.2(a).

c) The grammar of Exercise 4.2.2(c).

d) The grammar of Exercise 4.2.2(e).

e) The grammar of Exercise 4.2.2(g).

#### Answer

1. S -> S S + | S S * | a
    1. Left-factoring
        
            S -> S S A | a
            A -> + | *
            
    2. Not suitable
    3. Eliminating left-recursion
            
            // initial status
            1）S -> S S A | a
            2) A -> + | *
            
            // i = 1
            1) S -> a B
            2) B -> S A B | ε
            3) A -> + | *
            
            // i = 2, j = 1
            1) S -> a B
            2) B -> a B A B | ε
            3) A -> + | *
            
            // i = 3, j = 1 ~ 2
            // nothing changed
            
     4. Suitable

2. S -> 0 S 1 | 0 1
    1. Left-factoring
    
            S -> 0 A
            A -> S 1 | 1
            
    2. Not suitable，indirect left-recursion
    3. Eliminating left-recursion
    
            // initial status
            1) S -> 0 A
            2) A -> S 1 | 1
            
            // i = 1
            // nothing changed
            
            // i = 2, j = 1
            1) S -> 0 A
            2) A -> 0 A 1 | 1
            
     4. Suitable

3. S -> S (S) S | ε
    1. left factoring not needed.
    2. Not suitable
    3. Eliminating left-recursion
    
            // initial status
            1) S -> S (S) S | ε
            
            // i = 1
            1) S -> A
            2) A -> (S) S A | ε
            
            // i = 2, j = 1
            // nothing changed
     4. Suitable

4. 	S -> (L) | a
	L -> L, S | S
	
    1. left factoring not needed.
    2. Not suitable
    3. Eliminating left-recursion
    
            // initial status
            1) S -> (L) | a
            2) L -> L, S | S
            
            // i = 1
            // nothing changed
            
            // i = 2, j = 1
            1) S -> (L) | a
            2) L -> (L) A | a A
            3) A -> , S A | ε
            
            // i = 3, j = 1~2
            // nothing changed
      
      4. Suitable

### 4.3.3 ！

The following grammar is proposed to remove the "dangling else ambiguity" discussed in Section 4.3.2:

    stmt -> if expr then stmt
          | matchedStmt
    matchedStmt -> if expr then matchedStmt else stmt
                 | other
 
Show that this grammar is still ambiguous.

#### Answer

Indentation here specifies the matching if-then-elses.

    if expr 
    then 
        if expr 
        then matchedStmt 
        else
            if expr
            then matchedStmt
    else stmt

But this code can also be parsed into

    if expr 
    then 
        if expr 
        then matchedStmt 
        else
            if expr
            then matchedStmt
            else stmt
            
So this is still an ambiguous grammar. the reason is that in `matchedStmt -> if expr then matchedStmt else stmt`, the last `stmt`, if it contains another  `else` statement, can be considered to belong to the latter statement or to the statement containing the `matchedStmt` statement.